experiments: compute the state/allocation

coq_translation/examples-from-rust-book/MonadExperiments.v
@@ -26,25 +26,6 @@ Module State.
         read a1 (write a2 s v2) = read a1 s;
       }.
   End Valid.
-(* 
-Module ReadWriteSemantics.
-  Record t {State Address : Set} : Type := {
-    read {A : Set} : Address -> State -> A -> Prop;
-    write {A : Set} : Address -> State -> A -> State -> Prop;
-  }.
-
-  Module Valid.
-    Record t {State Address : Set} (S : @ReadWriteSemantics.t State Address)
-      : Prop := {
-      same (a : Address) {A : Set} (s s' : State) (v : A) :
-        S.(write) a s v s' ->
-        S.(read) a s' v;
-      different (a1 a2 : Address) {A1 A2 : Set} (s : State) :
-        a1 <> a2 ->
-        S.(read) a1 s v1 ->
-
-    }.
-  End Valid. *)
 End State.
 
 Module Allocation.
@@ -63,56 +44,8 @@ Module Allocation.
   Definition get {Address : Set} (allocation : t Address) (index : nat)
     : option Address :=
     get_rev (List.rev allocation) index.
-  Arguments get /.
 End Allocation.
 Definition Allocation := Allocation.t.
-
-(* Module Zone.
-  Class Trait (Self Address : Set) : Type := {
-    zero : Self;
-    add : Self -> Address -> option Self;
-    is_in : Address -> Self -> Prop;
-  }.
-
-  Fixpoint sum `{Trait} (allocation : Allocation Address) : option Self :=
-    match allocation with
-    | [] => Some zero
-    | None :: allocation => sum allocation
-    | Some address :: allocation =>
-      match sum allocation with
-      | Some zone => add zone address
-      | None => None
-      end
-    end.
-
-  Module Valid.
-    Record t `(Trait) : Prop := {
-      is_in_after_add zone address zone' :
-        add zone address = Some zone' ->
-        is_in address zone';
-      is_not_in_before_add zone address zone' :
-        add zone address = Some zone' ->
-        ~ is_in address zone;
-    }.
-  End Valid.
-
-  Lemma summable_implies_uniq `{T : Trait}
-    (allocation : Allocation Address) (zone : Self) :
-    Valid.t T ->
-    sum allocation = Some zone ->
-    forall index1 index2,
-    index1 <> index2 ->
-    match
-      Allocation.get allocation index1,
-      Allocation.get allocation index2
-    with
-    | Some address1, Some address2 =>
-      address1 <> address2
-    | _, _ => True
-    end.
-  Proof.
-  Admitted.
-End Zone. *)
 
 Module M.
   Inductive t : Set -> Set :=
@@ -129,7 +62,208 @@ Notation "'let*' x ':=' e1 'in' e2" :=
   (M.Bind e1 (fun x => e2))
   (at level 200, x name, e1 at level 100, e2 at level 200).
 
+Module M_State.
+  Inductive t (Address A : Set) : Set :=
+  | Pure : A -> t Address A
+  | Bind {B : Set} : t Address B -> (B -> t Address A) -> t Address A
+  | GetAddress : (Address -> t Address A) -> t Address A
+  | Cast {B B' : Set} : B -> (B' -> t Address A) -> t Address A
+  | Impossible : t Address A.
+  Arguments Pure {_ _}.
+  Arguments Bind {_ _ _}.
+  Arguments GetAddress {_ _}.
+  Arguments Cast {_ _ _ _}.
+  Arguments Impossible {_ _}.
+End M_State.
+Definition M_State := M_State.t.
+
+Fixpoint run_state {State Address A : Set} `{State.Trait State Address}
+  (fuel : nat) (allocation : Allocation Address) (s : State)
+  (e : M A) {struct fuel} :
+  M_State Address (A * Allocation Address * State) :=
+  match fuel with
+  | O => M_State.Impossible
+  | S fuel =>
+    match e with
+    | M.Pure v =>
+      M_State.Pure (v, allocation, s)
+    | M.Bind e1 e2 =>
+      M_State.Bind
+        (run_state fuel allocation s e1) (fun '(v1, allocation, s) =>
+        run_state fuel allocation s (e2 v1))
+    | M.Loop body is_break as e =>
+      M_State.Bind
+      (run_state fuel allocation s body) (fun '(v, allocation, s) =>
+      if is_break v then
+        M_State.Pure (v, allocation, s)
+      else
+        run_state fuel allocation s e)
+    | M.Malloc v =>
+      M_State.GetAddress (fun address =>
+      (* Check that the address was not yet allocated *)
+      match State.read address s with
+      | None =>
+        let index := List.length allocation in
+        let allocation := Some address :: allocation in
+        M_State.Cast v (fun v =>
+        let s := State.write address s v in
+        (* Check that the address is now allocated *)
+        match State.read address s with
+        | Some _ =>
+          M_State.Pure (index, allocation, s)
+        | None => M_State.Impossible
+        end)
+      | Some _ => M_State.Impossible
+      end)
+    | M.Read index =>
+      match Allocation.get allocation index with
+      | Some address =>
+        match State.read address s with
+        | Some v =>
+          M_State.Cast v (fun v =>
+          M_State.Pure (v, allocation, s))
+        | None => M_State.Impossible
+        end
+      | None => M_State.Impossible
+      end
+    | M.Write index v =>
+      match Allocation.get allocation index with
+      | Some address =>
+        M_State.Cast v (fun v =>
+        let s := State.write address s v in
+        M_State.Pure (tt, allocation, s))
+      | None => M_State.Impossible
+      end
+    end
+  end.
+
 Module Run.
+  Inductive t {Address A : Set} : M_State Address A -> A -> Prop :=
+  | Pure (v : A) : t (M_State.Pure v) v
+  | Bind {B : Set} (e1 : M_State Address B) (e2 : B -> M_State Address A)
+      (v1 : B) (v2 : A) :
+    t e1 v1 ->
+    t (e2 v1) v2 ->
+    t (M_State.Bind e1 e2) v2
+  | GetAddress (f : Address -> M_State Address A) (address : Address) (v : A) :
+    t (f address) v ->
+    t (M_State.GetAddress f) v
+  | Cast {B : Set} (v : B) (f : B -> M_State Address A) (v' : A) :
+    t (f v) v' ->
+    t (M_State.Cast v f) v'.
+End Run.
+
+Module Example.
+  (** Code for:
+      fn main() {
+        let mut x = 5;
+        let mut y = 10;
+        let mut z = 15;
+        let s1 = x + y + z;
+        
+        x = 50;
+        y = 100;
+        z = 150;
+        let s2 = x + y + z;
+        
+        return s1 + s2;
+      }
+  *)
+  Definition main : M Z :=
+    let* x := M.Malloc 5 in
+    let* y := M.Malloc 10 in
+    let* z := M.Malloc 15 in
+    let* v_x := M.Read x in
+    let* v_y := M.Read y in
+    let* v_z := M.Read z in
+    let s1 := v_x + v_y + v_z in
+    let* _ := M.Write x 50 in
+    let* _ := M.Write y 100 in
+    let* _ := M.Write z 150 in
+    let* v_x := M.Read x in
+    let* v_y := M.Read y in
+    let* v_z := M.Read z in
+    let s2 := v_x + v_y + v_z in
+    M.Pure (s1 + s2).
+
+  Module State.
+    Record t : Set := {
+      x : option Z;
+      y : option Z;
+      z : option Z;
+    }.
+
+    Definition init : t := {|
+      x := None;
+      y := None;
+      z := None;
+    |}.
+  End State.
+  Definition State := State.t.
+
+  Module Address.
+    Inductive t : Set :=
+    | X
+    | Y
+    | Z.
+  End Address.
+  Definition Address := Address.t.
+
+  Global Instance State_Trait : State.Trait State Address := {
+    get_Set _ := Z;
+    read address state :=
+      match address with
+      | Address.X => state.(State.x)
+      | Address.Y => state.(State.y)
+      | Address.Z => state.(State.z)
+      end;
+    write address state value :=
+      match address with
+      | Address.X => {| State.x := Some value; State.y := state.(State.y); State.z := state.(State.z) |}
+      | Address.Y => {| State.x := state.(State.x); State.y := Some value; State.z := state.(State.z) |}
+      | Address.Z => {| State.x := state.(State.x); State.y := state.(State.y); State.z := Some value |}
+      end;
+  }.
+
+  Ltac run_malloc a :=
+    eapply Run.GetAddress with (address := a);
+    apply Run.Cast;
+    apply Run.Pure.
+
+  Definition is_all_allocated (s : State) : Prop :=
+    forall address,
+    State.read address s <> None.
+
+  Lemma run_main :
+    exists allocation s,
+    Run.t (run_state 1000 [] State.init main) (330, allocation, s) /\
+    is_all_allocated s.
+  Proof.
+    repeat eexists.
+    { unfold main.
+      eapply Run.Bind. {
+        run_malloc Address.X.
+      }
+      eapply Run.Bind. {
+        run_malloc Address.Y.
+      }
+      eapply Run.Bind. {
+        run_malloc Address.Z.
+      }
+      repeat (eapply Run.Bind; [
+        apply Run.Cast;
+        apply Run.Pure
+      |]).
+      apply Run.Pure.
+    }
+    { simpl.
+      unfold is_all_allocated.
+      now intros [].
+    }
+  Qed.
+End Example.
+
+(*Module Run.
   Inductive t {State Address : Set} `{State.Trait State Address}
     (allocation : Allocation Address) (s : State) :
     forall {A : Set},
@@ -308,3 +442,4 @@ Module Example.
     { apply Run.Pure. }
   Qed.
 End Example.
+*)
